theories/NewSmallStep/Typing/Resolve.v
@@ -1,5 +1,7 @@
 From Stdlib Require Import List.
+From Stdlib Require Import Program.Equality.
 
+Require Import theories.NewSmallStep.Core.Effects.
 Require Import theories.NewSmallStep.Core.Syntax.
 Require Import theories.NewSmallStep.Core.Values.
 Require Import theories.NewSmallStep.Typing.Types.
@@ -9,7 +11,73 @@ Import ListNotations.
 Inductive NResolvedRegionExpr : RegionExpr -> Prop :=
 | NRR_Const :
     forall r,
-      NResolvedRegionExpr (RConst r).
+      NResolvedRegionExpr (region_const_expr r).
+
+Inductive NResolvedRegionType : RegionType -> Prop :=
+| NRRT_Const :
+    forall r,
+      NResolvedRegionType (region_const_type r)
+| NRRT_BVar :
+    forall n,
+      NResolvedRegionType (Rgn_BVar true true n).
+
+Inductive NResolveRegionType :
+    Rho -> RegionType -> RegionType -> Prop :=
+| NResolveRegion_Const :
+    forall rho r,
+      NResolveRegionType rho (region_const_type r) (region_const_type r)
+| NResolveRegion_FVar :
+    forall rho x r,
+      rho_lookup x rho = Some r ->
+      NResolveRegionType rho (Rgn_FVar true true x) (region_const_type r)
+| NResolveRegion_BVar :
+    forall rho n,
+      NResolveRegionType rho
+        (Rgn_BVar true true n)
+        (Rgn_BVar true true n).
+
+Inductive NResolvedStaticAction : StaticAction -> Prop :=
+| NRSA_Alloc :
+    forall rgn,
+      NResolvedRegionType rgn ->
+      NResolvedStaticAction (SAlloc rgn)
+| NRSA_Read :
+    forall rgn,
+      NResolvedRegionType rgn ->
+      NResolvedStaticAction (SRead rgn)
+| NRSA_Write :
+    forall rgn,
+      NResolvedRegionType rgn ->
+      NResolvedStaticAction (SWrite rgn).
+
+Definition NResolvedStaticEffect (eff : StaticEffect) : Prop :=
+  Forall NResolvedStaticAction eff.
+
+Inductive NResolveStaticAction :
+    Rho -> StaticAction -> StaticAction -> Prop :=
+| NResolve_SAlloc :
+    forall rho rgn rgn',
+      NResolveRegionType rho rgn rgn' ->
+      NResolveStaticAction rho (SAlloc rgn) (SAlloc rgn')
+| NResolve_SRead :
+    forall rho rgn rgn',
+      NResolveRegionType rho rgn rgn' ->
+      NResolveStaticAction rho (SRead rgn) (SRead rgn')
+| NResolve_SWrite :
+    forall rho rgn rgn',
+      NResolveRegionType rho rgn rgn' ->
+      NResolveStaticAction rho (SWrite rgn) (SWrite rgn').
+
+Inductive NResolveStaticEffect :
+    Rho -> StaticEffect -> StaticEffect -> Prop :=
+| NResolveStaticEffect_Nil :
+    forall rho,
+      NResolveStaticEffect rho [] []
+| NResolveStaticEffect_Cons :
+    forall rho action action' eff eff',
+      NResolveStaticAction rho action action' ->
+      NResolveStaticEffect rho eff eff' ->
+      NResolveStaticEffect rho (action :: eff) (action' :: eff').
 
 Inductive NResolvedTy : NTy -> Prop :=
 | NRTy_Nat :
@@ -21,17 +89,22 @@ Inductive NResolvedTy : NTy -> Prop :=
 | NRTy_Effect :
     NResolvedTy TyEffect
 | NRTy_Ref :
-    forall r ty,
+    forall rgn ty,
+      NResolvedRegionType rgn ->
       NResolvedTy ty ->
-      NResolvedTy (TyRef (RConst r) ty)
+      NResolvedTy (TyRef rgn ty)
 | NRTy_Arrow :
     forall ty_arg eff_body ty_body eff_summary,
       NResolvedTy ty_arg ->
+      NResolvedStaticEffect eff_body ->
       NResolvedTy ty_body ->
+      NResolvedStaticEffect eff_summary ->
       NResolvedTy (TyArrow ty_arg eff_body ty_body eff_summary)
 | NRTy_ForallRgn :
-    forall x ty,
-      NResolvedTy (TyForallRgn x ty).
+    forall eff ty,
+      NResolvedStaticEffect eff ->
+      NResolvedTy ty ->
+      NResolvedTy (TyForallRgn eff ty).
 
 Inductive NResolveTy : Rho -> NTy -> NTy -> Prop :=
 | NResolve_Nat :
@@ -47,20 +120,54 @@ Inductive NResolveTy : Rho -> NTy -> NTy -> Prop :=
     forall rho,
       NResolveTy rho TyEffect TyEffect
 | NResolve_Ref :
-    forall rho rgn ty ty' r,
-      eval_region rho rgn = Some r ->
+    forall rho rgn rgn' ty ty',
+      NResolveRegionType rho rgn rgn' ->
       NResolveTy rho ty ty' ->
-      NResolveTy rho (TyRef rgn ty) (TyRef (RConst r) ty')
+      NResolveTy rho (TyRef rgn ty) (TyRef rgn' ty')
 | NResolve_Arrow :
-    forall rho ty_arg ty_arg' eff_body ty_body ty_body' eff_summary,
+    forall rho ty_arg ty_arg' eff_body eff_body'
+      ty_body ty_body' eff_summary eff_summary',
       NResolveTy rho ty_arg ty_arg' ->
+      NResolveStaticEffect rho eff_body eff_body' ->
       NResolveTy rho ty_body ty_body' ->
+      NResolveStaticEffect rho eff_summary eff_summary' ->
       NResolveTy rho
         (TyArrow ty_arg eff_body ty_body eff_summary)
-        (TyArrow ty_arg' eff_body ty_body' eff_summary)
+        (TyArrow ty_arg' eff_body' ty_body' eff_summary')
 | NResolve_ForallRgn :
-    forall rho x ty,
-      NResolveTy rho (TyForallRgn x ty) (TyForallRgn x ty).
+    forall rho eff eff' ty ty',
+      NResolveStaticEffect rho eff eff' ->
+      NResolveTy rho ty ty' ->
+      NResolveTy rho (TyForallRgn eff ty) (TyForallRgn eff' ty').
+
+Lemma NResolveRegionType_resolved :
+  forall rho rgn rgn',
+    NResolveRegionType rho rgn rgn' ->
+    NResolvedRegionType rgn'.
+Proof.
+  intros rho rgn rgn' HResolve.
+  inversion HResolve; subst; constructor.
+Qed.
+
+Lemma NResolveStaticAction_resolved :
+  forall rho action action',
+    NResolveStaticAction rho action action' ->
+    NResolvedStaticAction action'.
+Proof.
+  intros rho action action' HResolve.
+  inversion HResolve; subst; constructor;
+    eauto using NResolveRegionType_resolved.
+Qed.
+
+Lemma NResolveStaticEffect_resolved :
+  forall rho eff eff',
+    NResolveStaticEffect rho eff eff' ->
+    NResolvedStaticEffect eff'.
+Proof.
+  intros rho eff eff' HResolve.
+  induction HResolve; constructor;
+    eauto using NResolveStaticAction_resolved.
+Qed.
 
 Lemma NResolveTy_resolved :
   forall rho ty ty',
@@ -68,21 +175,83 @@ Lemma NResolveTy_resolved :
     NResolvedTy ty'.
 Proof.
   intros rho ty ty' HResolve.
-  induction HResolve; constructor; assumption.
+  induction HResolve; constructor;
+    eauto using NResolveRegionType_resolved,
+      NResolveStaticEffect_resolved.
 Qed.
 
 Lemma NResolveTy_ref_inv :
   forall rho rgn ty ty_resolved,
     NResolveTy rho (TyRef rgn ty) ty_resolved ->
-    exists r ty',
-      eval_region rho rgn = Some r /\
+    exists rgn' ty',
+      NResolveRegionType rho rgn rgn' /\
       NResolveTy rho ty ty' /\
-      ty_resolved = TyRef (RConst r) ty'.
+      ty_resolved = TyRef rgn' ty'.
 Proof.
   intros rho rgn ty ty_resolved HResolve.
   inversion HResolve; subst.
-  exists r, ty'.
+  exists rgn', ty'.
   repeat split; assumption || reflexivity.
+Qed.
+
+Lemma NResolveRegionType_deterministic :
+  forall rho rgn rgn1 rgn2,
+    NResolveRegionType rho rgn rgn1 ->
+    NResolveRegionType rho rgn rgn2 ->
+    rgn1 = rgn2.
+Proof.
+  intros rho rgn rgn1 rgn2 HLeft HRight.
+  inversion HLeft; subst; inversion HRight; subst;
+    try reflexivity.
+  match goal with
+  | H1 : rho_lookup ?x ?rho = Some ?r1,
+    H2 : rho_lookup ?x ?rho = Some ?r2 |- _ =>
+      rewrite H1 in H2; inversion H2; reflexivity
+  end.
+Qed.
+
+Lemma NResolveStaticAction_deterministic :
+  forall rho action action1 action2,
+    NResolveStaticAction rho action action1 ->
+    NResolveStaticAction rho action action2 ->
+    action1 = action2.
+Proof.
+  intros rho action action1 action2 HLeft HRight.
+  inversion HLeft; subst; inversion HRight; subst;
+    match goal with
+    | H1 : NResolveRegionType rho ?rgn ?rgn1,
+      H2 : NResolveRegionType rho ?rgn ?rgn2 |- _ =>
+        pose proof
+          (NResolveRegionType_deterministic rho rgn rgn1 rgn2 H1 H2);
+        subst
+    end;
+    reflexivity.
+Qed.
+
+Lemma NResolveStaticEffect_deterministic :
+  forall rho eff eff1 eff2,
+    NResolveStaticEffect rho eff eff1 ->
+    NResolveStaticEffect rho eff eff2 ->
+    eff1 = eff2.
+Proof.
+  intros rho eff eff1 eff2 HLeft.
+  revert eff2.
+  induction HLeft; intros eff2 HRight.
+  - inversion HRight; reflexivity.
+  - inversion HRight; subst.
+    match goal with
+    | H1 : NResolveStaticAction rho action action',
+      H2 : NResolveStaticAction rho action ?action_other |- _ =>
+        pose proof
+          (NResolveStaticAction_deterministic
+            rho action action' action_other H1 H2);
+        subst action_other
+    end.
+    match goal with
+    | HRest : NResolveStaticEffect rho eff ?eff_other |- _ =>
+        specialize (IHHLeft _ HRest); subst
+    end.
+    reflexivity.
 Qed.
 
 Lemma NResolveTy_deterministic :
@@ -97,8 +266,11 @@ Proof.
     try solve [inversion HRight; subst; reflexivity].
   - destruct
       (NResolveTy_ref_inv rho rgn ty ty_right HRight)
-      as (r_other & ty_other & HRgnOther & HTyOther & ->).
-    rewrite H in HRgnOther. inversion HRgnOther; subst.
+      as (rgn_other & ty_other & HRgnOther & HTyOther & ->).
+    pose proof
+      (NResolveRegionType_deterministic
+        rho rgn rgn' rgn_other H HRgnOther);
+      subst rgn_other.
     specialize (IHHLeft _ HTyOther). subst.
     reflexivity.
   - inversion HRight; subst.
@@ -108,18 +280,87 @@ Proof.
       HResolve : NResolveTy ?rho ?ty ?resolved_other |- _ =>
         specialize (IH _ HResolve); subst
     end.
+    match goal with
+    | HLeftEff : NResolveStaticEffect rho eff_body eff_body',
+      HRightEff : NResolveStaticEffect rho eff_body ?eff_body_other
+      |- TyArrow _ eff_body' _ _ = TyArrow _ ?eff_body_other _ _ =>
+        pose proof
+          (NResolveStaticEffect_deterministic
+            rho eff_body eff_body' eff_body_other HLeftEff HRightEff);
+        subst eff_body_other
+    end.
+    match goal with
+    | HLeftEff : NResolveStaticEffect rho eff_summary eff_summary',
+      HRightEff : NResolveStaticEffect rho eff_summary ?eff_summary_other
+      |- TyArrow _ _ _ eff_summary' = TyArrow _ _ _ ?eff_summary_other =>
+        pose proof
+          (NResolveStaticEffect_deterministic
+            rho eff_summary eff_summary' eff_summary_other
+            HLeftEff HRightEff);
+        subst eff_summary_other
+    end.
     subst. reflexivity.
+  - inversion HRight; subst.
+    repeat match goal with
+    | IH : forall ty_res : NTy,
+        NResolveTy ?rho ?ty ty_res -> ?resolved = ty_res,
+      HResolve : NResolveTy ?rho ?ty ?resolved_other |- _ =>
+        specialize (IH _ HResolve); subst
+    end.
+    match goal with
+    | HLeftEff : NResolveStaticEffect rho eff eff',
+      HRightEff : NResolveStaticEffect rho eff ?eff_other
+      |- TyForallRgn eff' _ = TyForallRgn ?eff_other _ =>
+        pose proof
+          (NResolveStaticEffect_deterministic
+            rho eff eff' eff_other HLeftEff HRightEff);
+        subst eff_other
+    end.
+    subst.
+    reflexivity.
+Qed.
+
+Lemma NResolveRegionType_const_eval :
+  forall rho rgn r,
+    NResolveRegionType rho rgn (region_const_type r) ->
+    eval_region_type rho rgn = Some r.
+Proof.
+  intros rho rgn r HResolve.
+  inversion HResolve; subst; try reflexivity.
+  assumption.
+Qed.
+
+Lemma NResolveRegionType_region_to_type :
+  forall idx rho (rgn : Region idx) r,
+    eval_region_any rho rgn = Some r ->
+    NResolveRegionType rho (region_to_type rgn) (region_const_type r).
+Proof.
+  intros idx rho rgn r HResolve.
+  destruct rgn; simpl in HResolve.
+  - inversion HResolve; subst. constructor.
+  - econstructor. exact HResolve.
+  - inversion HResolve.
+Qed.
+
+Lemma NResolveRegionType_region_expr_to_type :
+  forall rho rgn r,
+    eval_region rho rgn = Some r ->
+    NResolveRegionType rho (region_expr_to_type rgn) (region_const_type r).
+Proof.
+  intros rho rgn r HResolve.
+  apply NResolveRegionType_region_to_type.
+  exact HResolve.
 Qed.
 
 Lemma NResolveTy_ref_same_region :
   forall rho rgn ty r ty',
-    NResolveTy rho (TyRef rgn ty) (TyRef (RConst r) ty') ->
-    eval_region rho rgn = Some r.
+    NResolveTy rho (TyRef rgn ty) (TyRef (region_const_type r) ty') ->
+    eval_region_type rho rgn = Some r.
 Proof.
   intros rho rgn ty r ty' HResolve.
   destruct
-    (NResolveTy_ref_inv rho rgn ty (TyRef (RConst r) ty') HResolve)
-    as (r0 & ty0 & HRgn & _ & HEq).
+    (NResolveTy_ref_inv rho rgn ty (TyRef (region_const_type r) ty') HResolve)
+    as (rgn0 & ty0 & HRgn & _ & HEq).
   inversion HEq; subst.
-  assumption.
+  eapply NResolveRegionType_const_eval; eauto.
 Qed.
