theories/NewSmallStep/Typing/Types.v
@@ -1,3 +1,5 @@
+From Stdlib Require Import Ascii.
+
 Require Import theories.NewSmallStep.Core.Effects.
 Require Import theories.NewSmallStep.Core.Syntax.
 
@@ -6,6 +8,76 @@ Inductive NTy :=
 | TyBool : NTy
 | TyUnit : NTy
 | TyEffect : NTy
-| TyRef : RegionExpr -> NTy -> NTy
+| TyRef : RegionType -> NTy -> NTy
 | TyArrow : NTy -> StaticEffect -> NTy -> StaticEffect -> NTy
-| TyForallRgn : VarId -> NTy -> NTy.
+| TyForallRgn : StaticEffect -> NTy -> NTy.
+
+Fixpoint open_ty_at (k : nat) (u : RegionType) (ty : NTy) : NTy :=
+  match ty with
+  | TyNat => TyNat
+  | TyBool => TyBool
+  | TyUnit => TyUnit
+  | TyEffect => TyEffect
+  | TyRef rgn ty_inner =>
+      TyRef (open_region_type_at k u rgn) (open_ty_at k u ty_inner)
+  | TyArrow ty_arg eff_body ty_body eff_summary =>
+      TyArrow
+        (open_ty_at k u ty_arg)
+        (open_static_effect_at k u eff_body)
+        (open_ty_at k u ty_body)
+        (open_static_effect_at k u eff_summary)
+  | TyForallRgn eff ty_body =>
+      TyForallRgn
+        (open_static_effect_at (S k) u eff)
+        (open_ty_at (S k) u ty_body)
+  end.
+
+Definition open_ty_type (u : RegionType) (ty : NTy) : NTy :=
+  open_ty_at 0 u ty.
+
+Definition open_ty (rgn : RegionExpr) (ty : NTy) : NTy :=
+  open_ty_type (region_expr_to_type rgn) ty.
+
+Fixpoint close_ty_at (k : nat) (x : VarId) (ty : NTy) : NTy :=
+  match ty with
+  | TyNat => TyNat
+  | TyBool => TyBool
+  | TyUnit => TyUnit
+  | TyEffect => TyEffect
+  | TyRef rgn ty_inner =>
+      TyRef (close_region_type_at k x rgn) (close_ty_at k x ty_inner)
+  | TyArrow ty_arg eff_body ty_body eff_summary =>
+      TyArrow
+        (close_ty_at k x ty_arg)
+        (close_static_effect_at k x eff_body)
+        (close_ty_at k x ty_body)
+        (close_static_effect_at k x eff_summary)
+  | TyForallRgn eff ty_body =>
+      TyForallRgn
+        (close_static_effect_at (S k) x eff)
+        (close_ty_at (S k) x ty_body)
+  end.
+
+Definition close_ty (x : VarId) (ty : NTy) : NTy :=
+  close_ty_at 0 x ty.
+
+Fixpoint subst_ty (x : VarId) (replacement : RegionExpr) (ty : NTy) : NTy :=
+  match ty with
+  | TyNat => TyNat
+  | TyBool => TyBool
+  | TyUnit => TyUnit
+  | TyEffect => TyEffect
+  | TyRef rgn ty_inner =>
+      TyRef (subst_region_type x replacement rgn)
+        (subst_ty x replacement ty_inner)
+  | TyArrow ty_arg eff_body ty_body eff_summary =>
+      TyArrow
+        (subst_ty x replacement ty_arg)
+        (subst_static_effect x replacement eff_body)
+        (subst_ty x replacement ty_body)
+        (subst_static_effect x replacement eff_summary)
+  | TyForallRgn eff ty_body =>
+      TyForallRgn
+        (subst_static_effect x replacement eff)
+        (subst_ty x replacement ty_body)
+  end.
