theories/NewSmallStep/Typing/Judgments.v
@@ -1,5 +1,6 @@
 From Stdlib Require Import List.
-From Stdlib Require Import String.
+From Stdlib Require Import Ascii.
+From Stdlib Require Import Program.Equality.
 
 Require Import theories.NewSmallStep.Core.Effects.
 Require Import theories.NewSmallStep.Core.Syntax.
@@ -14,7 +15,7 @@ Fixpoint ctx_lookup (x : VarId) (gamma : NCtx) : option NTy :=
   match gamma with
   | [] => None
   | (y, ty) :: gamma' =>
-      if String.eqb x y then Some ty else ctx_lookup x gamma'
+      if ascii_dec x y then Some ty else ctx_lookup x gamma'
   end.
 
 Definition ctx_binds (x : VarId) (ty : NTy) (gamma : NCtx) : Prop :=
@@ -26,11 +27,14 @@ Definition static_union (eff1 eff2 : StaticEffect) : StaticEffect :=
 Definition static_readonly (eff : StaticEffect) : Prop :=
   forall r, ~ In (SWrite r) eff.
 
-Definition region_expr_wf (omega : NRgnCtx) (rgn : RegionExpr) : Prop :=
-  match rgn with
-  | RConst _ => True
-  | RVar x => In x omega
-  end.
+Inductive region_expr_wf : NRgnCtx -> RegionExpr -> Prop :=
+| REWF_Const :
+    forall omega r,
+      region_expr_wf omega (region_const_expr r)
+| REWF_FVar :
+    forall omega x,
+      In x omega ->
+      region_expr_wf omega (region_var_expr x).
 
 Inductive NTcExp : NCtx -> NRgnCtx -> NExpr -> NTy -> StaticEffect -> Prop :=
 | NT_Const :
@@ -55,8 +59,10 @@ Inductive NTcExp : NCtx -> NRgnCtx -> NExpr -> NTy -> StaticEffect -> Prop :=
         (TyArrow ty_arg eff_body ty_body eff_summary) []
 | NT_LambdaRgn :
     forall gamma omega x e ty eff,
+      NBackTriangle gamma (x :: omega) e EEmpty ->
       NTcExp gamma (x :: omega) e ty eff ->
-      NTcExp gamma omega (ELambdaRgn x e) (TyForallRgn x ty) []
+      NTcExp gamma omega (ELambdaRgn x e)
+        (TyForallRgn (close_static_effect x eff) (close_ty x ty)) []
 | NT_MuApp :
     forall gamma omega ef ea ty_arg ty_body eff_body eff_summary eff_f eff_a,
       NTcExp gamma omega ef
@@ -65,10 +71,11 @@ Inductive NTcExp : NCtx -> NRgnCtx -> NExpr -> NTy -> StaticEffect -> Prop :=
       NTcExp gamma omega (EMuApp ef ea) ty_body
         (static_union eff_f (static_union eff_a eff_body))
 | NT_RgnApp :
-    forall gamma omega er r x ty eff_f,
+    forall gamma omega er r ty eff_body eff_f,
       region_expr_wf omega r ->
-      NTcExp gamma omega er (TyForallRgn x ty) eff_f ->
-      NTcExp gamma omega (ERgnApp er r) ty eff_f
+      NTcExp gamma omega er (TyForallRgn eff_body ty) eff_f ->
+      NTcExp gamma omega (ERgnApp er r) (open_ty r ty)
+        (static_union eff_f (open_static_effect r eff_body))
 | NT_EffApp :
     forall gamma omega ef ea ty_arg ty_body eff_body eff_summary eff_f eff_a,
       NTcExp gamma omega ef
@@ -87,21 +94,21 @@ Inductive NTcExp : NCtx -> NRgnCtx -> NExpr -> NTy -> StaticEffect -> Prop :=
     forall gamma omega r e ty eff,
       region_expr_wf omega r ->
       NTcExp gamma omega e ty eff ->
-      NTcExp gamma omega (ERef r e) (TyRef r ty)
-        (SAlloc 0 :: eff)
+      NTcExp gamma omega (ERef r e) (TyRef (region_expr_to_type r) ty)
+        (SAlloc (region_expr_to_type r) :: eff)
 | NT_Deref :
     forall gamma omega r e ty eff,
       region_expr_wf omega r ->
-      NTcExp gamma omega e (TyRef r ty) eff ->
+      NTcExp gamma omega e (TyRef (region_expr_to_type r) ty) eff ->
       NTcExp gamma omega (EDeref r e) ty
-        (SRead 0 :: eff)
+        (SRead (region_expr_to_type r) :: eff)
 | NT_Assign :
     forall gamma omega r ea ev ty eff_a eff_v,
       region_expr_wf omega r ->
-      NTcExp gamma omega ea (TyRef r ty) eff_a ->
+      NTcExp gamma omega ea (TyRef (region_expr_to_type r) ty) eff_a ->
       NTcExp gamma omega ev ty eff_v ->
       NTcExp gamma omega (EAssign r ea ev) TyUnit
-        (SWrite 0 :: static_union eff_a eff_v)
+        (SWrite (region_expr_to_type r) :: static_union eff_a eff_v)
 | NT_Plus :
     forall gamma omega e1 e2 eff1 eff2,
       NTcExp gamma omega e1 TyNat eff1 ->
@@ -153,4 +160,108 @@ Inductive NTcExp : NCtx -> NRgnCtx -> NExpr -> NTy -> StaticEffect -> Prop :=
       NTcExp gamma omega ETop TyEffect []
 | NT_Empty :
     forall gamma omega,
-      NTcExp gamma omega EEmpty TyEffect [].
+      NTcExp gamma omega EEmpty TyEffect []
+
+with NBackTriangle : NCtx -> NRgnCtx -> NExpr -> NExpr -> Prop :=
+| NBT_Num :
+    forall gamma omega n,
+      NTcExp gamma omega (EConst n) TyNat [] ->
+      NBackTriangle gamma omega (EConst n) EEmpty
+| NBT_Bool :
+    forall gamma omega b,
+      NTcExp gamma omega (EBool b) TyBool [] ->
+      NBackTriangle gamma omega (EBool b) EEmpty
+| NBT_Var :
+    forall gamma omega x ty,
+      NTcExp gamma omega (EVar x) ty [] ->
+      NBackTriangle gamma omega (EVar x) EEmpty
+| NBT_Mu :
+    forall gamma omega f x ec ee ty eff,
+      NTcExp gamma omega (EMu f x ec ee) ty eff ->
+      NBackTriangle gamma omega (EMu f x ec ee) EEmpty
+| NBT_LambdaRgn :
+    forall gamma omega x e ty eff,
+      NTcExp gamma omega (ELambdaRgn x e) ty eff ->
+      NBackTriangle gamma omega (ELambdaRgn x e) EEmpty
+| NBT_App :
+    forall gamma omega ef ea ty_mu eff_mu eff_eff
+      ty_ef ty_ea eff_ef eff_ea,
+      NTcExp gamma omega (EMuApp ef ea) ty_mu eff_mu ->
+      NTcExp gamma omega (EEffApp ef ea) TyEffect eff_eff ->
+      NTcExp gamma omega ef ty_ef eff_ef ->
+      NTcExp gamma omega ea ty_ea eff_ea ->
+      static_readonly eff_eff ->
+      static_readonly eff_ef ->
+      static_readonly eff_ea ->
+      NBackTriangle gamma omega ef (EEffApp ef ea) ->
+      NBackTriangle gamma omega ea (EEffApp ef ea) ->
+      NBackTriangle gamma omega (EMuApp ef ea) (EEffApp ef ea)
+| NBT_RgnApp :
+    forall gamma omega er r ty eff ty_app eff_app,
+      NTcExp gamma omega er ty eff ->
+      NTcExp gamma omega (ERgnApp er r) ty_app eff_app ->
+      NBackTriangle gamma omega er EEmpty ->
+      NBackTriangle gamma omega (ERgnApp er r) EEmpty
+| NBT_Cond :
+    forall gamma omega e et ef efft efff ty ty_t ty_f
+      eff_e eff_et eff_ef,
+      NTcExp gamma omega e TyBool eff_e ->
+      NTcExp gamma omega et ty_t eff_et ->
+      NTcExp gamma omega ef ty_f eff_ef ->
+      NTcExp gamma omega (ECond e et ef) ty
+        (static_union eff_e (static_union eff_et eff_ef)) ->
+      static_readonly eff_e ->
+      NBackTriangle gamma omega e EEmpty ->
+      NBackTriangle gamma omega et efft ->
+      NBackTriangle gamma omega ef efff ->
+      NBackTriangle gamma omega (ECond e et ef) (ECond e efft efff)
+| NBT_Ref :
+    forall gamma omega r e eff ty static ty_ref eff_ref,
+      NTcExp gamma omega e ty static ->
+      NTcExp gamma omega (ERef r e) ty_ref eff_ref ->
+      NBackTriangle gamma omega e eff ->
+      NBackTriangle gamma omega (ERef r e) (EConcat eff (EAllocAbs r))
+| NBT_Deref :
+    forall gamma omega r e eff ty static ty_deref eff_deref,
+      NTcExp gamma omega e ty static ->
+      NTcExp gamma omega (EDeref r e) ty_deref eff_deref ->
+      NBackTriangle gamma omega e eff ->
+      NBackTriangle gamma omega (EDeref r e) (EConcat eff (EReadAbs r))
+| NBT_Assign :
+    forall gamma omega r e1 e2 eff1 eff2 ty static ty_assign eff_assign,
+      NTcExp gamma omega e1 ty static ->
+      NTcExp gamma omega (EAssign r e1 e2) ty_assign eff_assign ->
+      static_readonly static ->
+      NBackTriangle gamma omega e1 eff1 ->
+      NBackTriangle gamma omega e2 eff2 ->
+      NBackTriangle gamma omega
+        (EAssign r e1 e2)
+        (EConcat eff1 (EConcat eff2 (EWriteAbs r)))
+| NBT_Plus :
+    forall gamma omega e1 e2 eff1 eff2 eff_static,
+      NTcExp gamma omega (EPlus e1 e2) TyNat eff_static ->
+      NBackTriangle gamma omega e1 eff1 ->
+      NBackTriangle gamma omega e2 eff2 ->
+      NBackTriangle gamma omega (EPlus e1 e2) (EConcat eff1 eff2)
+| NBT_Minus :
+    forall gamma omega e1 e2 eff1 eff2 eff_static,
+      NTcExp gamma omega (EMinus e1 e2) TyNat eff_static ->
+      NBackTriangle gamma omega e1 eff1 ->
+      NBackTriangle gamma omega e2 eff2 ->
+      NBackTriangle gamma omega (EMinus e1 e2) (EConcat eff1 eff2)
+| NBT_Times :
+    forall gamma omega e1 e2 eff1 eff2 eff_static,
+      NTcExp gamma omega (ETimes e1 e2) TyNat eff_static ->
+      NBackTriangle gamma omega e1 eff1 ->
+      NBackTriangle gamma omega e2 eff2 ->
+      NBackTriangle gamma omega (ETimes e1 e2) (EConcat eff1 eff2)
+| NBT_Eq :
+    forall gamma omega e1 e2 eff1 eff2 eff_static,
+      NTcExp gamma omega (EEq e1 e2) TyBool eff_static ->
+      NBackTriangle gamma omega e1 eff1 ->
+      NBackTriangle gamma omega e2 eff2 ->
+      NBackTriangle gamma omega (EEq e1 e2) (EConcat eff1 eff2)
+| NBT_Top :
+    forall gamma omega e ty eff,
+      NTcExp gamma omega e ty eff ->
+      NBackTriangle gamma omega e ETop.
